more content

DevconfCZ2025/6_Pos.lean
@@ -1,1 +1,55 @@
----
+-- Type classes
+
+-- # Positive numbers (Pos)
+
+-- https://lean-lang.org/functional_programming_in_lean/Overloading-and-Type-Classes/Positive-Numbers/#positive-numbers
+
+inductive Pos : Type where
+  | one : Pos
+  | succ : Pos → Pos
+
+def seven : Pos :=
+  Pos.succ (Pos.succ (Pos.succ (Pos.succ (Pos.succ (Pos.succ Pos.one)))))
+
+class Plus (α : Type) where
+  plus : α → α → α
+
+def Pos.plus : Pos → Pos → Pos
+  | Pos.one, k => Pos.succ k
+  | Pos.succ n, k => Pos.succ (n.plus k)
+
+instance : Plus Pos where
+  plus := Pos.plus
+
+open Plus (plus)
+
+def fourteen : Pos := plus seven seven
+
+instance : Add Pos where
+  add := Pos.plus
+
+example : Pos := seven + seven
+
+-- ToString class
+
+def posToString (atTop : Bool) (p : Pos) : String :=
+  let paren s := if atTop then s else "(" ++ s ++ ")"
+  match p with
+  | Pos.one => "Pos.one"
+  | Pos.succ n => paren s!"Pos.succ {posToString false n}"
+
+instance : ToString Pos where
+  toString := posToString true
+
+#eval IO.println s!"There are {seven}"
+
+-- convert to literals
+
+def Pos.toNat : Pos → Nat
+  | Pos.one => 1
+  | Pos.succ n => n.toNat + 1
+
+instance : ToString Pos where
+  toString x := toString (x.toNat)
+
+#eval s!"There are {seven}"
