git-status/Main.lean
@@ -1,0 +1,34 @@
+import Init.System.FilePath
+
+open System.FilePath
+
+def gitStatus (dir: System.FilePath) : IO Unit := do
+    let cfg :=
+      { cmd := "git"
+        args := #["status", "--short", "--untracked-files=no"]
+        cwd := dir
+      }
+    let out <- IO.Process.run cfg
+    if out.length > 0 then
+      let child <- IO.Process.spawn cfg
+      _ <- child.wait
+
+def checkDir (header _git: Bool) (dir: System.FilePath) : IO Unit := do
+  if (← dir.isDir) then
+    if (← (dir / ".git").isDir) then
+      if header then IO.println $ s!"\n# {dir}"
+      gitStatus dir
+
+open IO.FS.DirEntry in
+def main (args : List String) : IO Unit := do
+  let (ls,git) <-
+    if args.isEmpty then
+      let gitdir := System.FilePath.mk ".git"
+      if (← gitdir.isDir)
+      then pure (#[System.FilePath.mk "."],true)
+      else
+      let ents <- readDir "."
+      pure $ (ents.map path,false)
+    else pure (args.toArray.map System.FilePath.mk,false)
+  for f in ls do
+    checkDir (ls.size > 1) git f
