feline/README.md
@@ -1,0 +1,3 @@
+# feline
+
+Taken from https://lean-lang.org/functional_programming_in_lean/Hello___-World___/Worked-Example___--cat/
